\documentclass{article}
\usepackage{physics}
\usepackage{amsmath}
\begin{document}
\section{problem to stag central limit theorem}
\subsection{(a)}
we begin by considering that:
\begin{equation}
    \expval{(s-\expval{s})^{2}}=\expval{s^{2}-2s\expval{s}+\expval{s^{2}}} =\expval{s^{2}}-2\expval{s\expval{s}^{2}}
\end{equation}
we can now use the fact that: $\expval{s}$ and we can treat it as a constant and use the fact that expectation is a positive laner operator:
\begin{equation}
    \expval{(s-\expval{s})^{2}}=\expval{s^{2}}-2\expval{s}\expval{s}+\expval{s}^{2}\expval{1}=\expval{s^{2}}-\expval{2}=\sigma ^{2}
\end{equation}
\subsection{(b)}
\begin{equation}
    \expval{S_{n}}=\expval{\sum_{i=1}^{n} s_{i}}=\sum_{i=1}^{n} \expval{s_{i}}
\end{equation}
where we have used the fact that expectation is a positive linear operator.
\begin{equation}
    \expval{S_{n}}=\sum_{i=1}^{n} =\sum_{i=1}^{n-1} \expval{s_{i}}+\expval{s_{n}}=\expval{S_{n-2}}+2\expval{s}
\end{equation}
where we had used the recursive definition for $S_{n-1}$. 

\end{document}